add sub and neg and neg_one

src/defs.lean
@@ -1,7 +1,7 @@
-
 inductive term : Type
 | var : ℕ → term
 | zero : term
+| neg_one : term
 | one : term
 | and : term → term → term
 | or : term → term → term
@@ -9,12 +9,16 @@ inductive term : Type
 | not : term → term
 | ls : term → term
 | add : term → term → term
+| sub : term → term → term
+| neg : term → term
 
 open term
 
 def zero_seq : ℕ → bool := λ n, ff
 
 def one_seq : ℕ → bool := λ n, n = 0
+
+def neg_one_seq : ℕ → bool := λ n, tt
 
 def and_seq : Π (x y : ℕ → bool), ℕ → bool := λ x y n, x n && y n
 
@@ -37,15 +41,40 @@ def add_seq_aux (x y : ℕ → bool) : ℕ → bool × bool
 def add_seq (x y : ℕ → bool) : ℕ → bool :=
 λ n, (add_seq_aux x y n).1
 
+def sub_seq_aux (x y : ℕ → bool) : ℕ → bool × bool
+| 0 := (bxor (x 0) (y 0), bnot (x 0) && y 0)
+| (n+1) := let borrow := (sub_seq_aux n).2 in
+  let a := x (n + 1), b := y (n + 1) in
+  (bxor a (bxor b borrow), (bnot a && b) || ((bnot (bxor a b)) && borrow))
+
+def sub_seq (x y : ℕ → bool) : ℕ → bool :=
+λ n, (sub_seq_aux x y n).1
+
+def neg_seq_aux (x : ℕ → bool) : ℕ → bool × bool
+| 0 := (x 0, bnot (x 0))
+| (n+1) := let borrow := (neg_seq_aux n).2 in
+  let a := x (n + 1) in
+  (bxor (bnot a) borrow, bnot a && borrow)
+
+def neg_seq (x : ℕ → bool) : ℕ → bool :=
+λ n, (neg_seq_aux x n).1
+
 def term.eval : Π (t : term) (vars : ℕ → ℕ → bool), ℕ → bool
 | (var n) vars := vars n
 | zero vars := zero_seq
 | one vars := one_seq
+| neg_one vars := neg_one_seq
 | (and t₁ t₂) vars := and_seq (term.eval t₁ vars) (term.eval t₂ vars)
 | (or t₁ t₂) vars := or_seq (term.eval t₁ vars) (term.eval t₂ vars)
 | (xor t₁ t₂) vars := xor_seq (term.eval t₁ vars) (term.eval t₂ vars)
 | (not t) vars := not_seq (term.eval t vars)
 | (ls t) vars := ls_seq (term.eval t vars)
 | (add t₁ t₂) vars := add_seq (term.eval t₁ vars) (term.eval t₂ vars)
+| (sub t₁ t₂) vars := sub_seq (term.eval t₁ vars) (term.eval t₂ vars)
+| (neg t) vars := neg_seq (term.eval t vars)
 
 instance : has_add term := ⟨add⟩
+instance : has_sub term := ⟨sub⟩
+instance : has_one term := ⟨one⟩
+instance : has_zero term := ⟨zero⟩
+instance : has_neg term := ⟨neg⟩
